src/Assembly/Bounded.v
@@ -1,0 +1,732 @@
+Require Import Bedrock.Word Bedrock.Nomega.
+Require Import NPeano NArith PArith Ndigits ZArith Znat ZArith_dec Ndec.
+Require Import List Basics Bool Nsatz.
+
+Require Import Crypto.Assembly.QhasmUtil.
+Require Import Crypto.Assembly.WordizeUtil.
+Require Import Crypto.Assembly.Bounds.
+
+Import ListNotations.
+
+Section BoundedZ.
+
+  Section Trans4.
+    Definition min4 (a b c d: Z) :=
+      Z.min 0 (Z.min (Z.min a b) (Z.min c d)).
+
+    Definition max4 (a b c d: Z) :=
+      Z.max 0 (Z.max (Z.max a b) (Z.max c d)).
+
+    Ltac trans4min_tac := intros; unfold min4;
+      repeat match goal with
+      | [|- context[(Z.min ?x0 ?x1)%Z]] => is_var x1;
+        let A := fresh in let B := fresh in
+        destruct (Zmin_spec x0 x1)%Z as [A|A];
+        destruct A as [A B]; 
+        rewrite B; clear B
+      end; nomega.
+
+    Lemma trans4min_0: forall (x a b c d: Z),
+      (0 <= x)%Z -> (min4 a b c d <= x)%Z.
+    Proof. trans4min_tac. Qed.
+
+    Lemma trans4min_a: forall (x a b c d: Z),
+      (a <= x)%Z -> (min4 a b c d <= x)%Z.
+    Proof. trans4min_tac. Qed.
+
+    Lemma trans4min_b: forall (x a b c d: Z),
+      (b <= x)%Z -> (min4 a b c d <= x)%Z.
+    Proof. trans4min_tac. Qed.
+
+    Lemma trans4min_c: forall (x a b c d: Z),
+      (c <= x)%Z -> (min4 a b c d <= x)%Z.
+    Proof. trans4min_tac. Qed.
+
+    Lemma trans4min_d: forall (x a b c d: Z),
+      (d <= x)%Z -> (min4 a b c d <= x)%Z.
+    Proof. trans4min_tac. Qed.
+
+    Ltac trans4max_tac := intros; unfold max4;
+      repeat match goal with
+      | [|- context[(Z.max ?x0 ?x1)%Z]] => is_var x1;
+        let A := fresh in let B := fresh in
+        destruct (Zmax_spec x0 x1)%Z as [A|A];
+        destruct A as [A B]; 
+        rewrite B; clear B
+      end; try nomega.
+
+    Lemma trans4max_0: forall (x a b c d: Z),
+      (x <= 0)%Z -> (x <= max4 a b c d)%Z.
+    Proof. trans4max_tac. Qed.
+
+    Lemma trans4max_a: forall (x a b c d: Z),
+      (x <= a)%Z -> (x <= max4 a b c d)%Z.
+    Proof. trans4max_tac. Qed.
+
+    Lemma trans4max_b: forall (x a b c d: Z),
+      (x <= b)%Z -> (x <= max4 a b c d)%Z.
+    Proof. trans4max_tac. Qed.
+
+    Lemma trans4max_c: forall (x a b c d: Z),
+      (x <= c)%Z -> (x <= max4 a b c d)%Z.
+    Proof. trans4max_tac. Qed.
+
+    Lemma trans4max_d: forall (x a b c d: Z),
+      (x <= d)%Z -> (x <= max4 a b c d)%Z.
+    Proof. trans4max_tac. Qed.
+  End Trans4.
+
+  Section BoundedMul.
+    Lemma bZMul_min: forall (x0 low0 high0 x1 low1 high1: Z),
+      (low0 <= x0)%Z -> (x0 <= high0)%Z ->
+      (low1 <= x1)%Z -> (x1 <= high1)%Z ->
+      (min4 (low0 * low1) (low0 * high1)
+            (high0 * low1) (high0 * high1) <= x0 * x1)%Z.
+    Proof.
+      intros x0 low0 high0 x1 low1 high1
+        Hlow0 Hhigh0 Hlow1 Hhigh1.
+      destruct (Z_le_dec 0 x0), (Z_le_dec 0 x1).
+
+      - apply trans4min_0.
+        replace 0%Z with (0*0)%Z by nomega.
+        apply Z.mul_le_mono_nonneg; nomega.
+
+      - apply trans4min_c.
+        transitivity (x0 * low1)%Z.
+
+        + apply Z.mul_le_mono_nonpos_r; try nomega.
+        + apply Z.mul_le_mono_nonneg_l; try nomega.
+
+      - apply trans4min_b.
+        transitivity (x0 * high1)%Z.
+
+        + apply Z.mul_le_mono_nonneg_r; try nomega.
+        + apply Z.mul_le_mono_nonpos_l; try nomega.
+
+      - apply trans4min_0.
+        replace 0%Z with (0*0)%Z by nomega.
+        apply Z.mul_le_mono_nonpos; try nomega.
+    Qed.
+
+    Lemma bZMul_max: forall (x0 low0 high0 x1 low1 high1: Z),
+      (low0 <= x0)%Z -> (x0 <= high0)%Z ->
+      (low1 <= x1)%Z -> (x1 <= high1)%Z ->
+      (x0 * x1 <=
+      max4 (low0 * low1) (low0 * high1)
+           (high0 * low1) (high0 * high1))%Z.
+    Proof.
+      intros x0 low0 high0 x1 low1 high1
+        Hlow0 Hhigh0 Hlow1 Hhigh1.
+      destruct (Z_le_dec 0 x0), (Z_le_dec 0 x1).
+
+      - apply trans4max_d.
+        apply Z.mul_le_mono_nonneg; nomega.
+
+      - apply trans4max_0.
+        replace 0%Z with (0*0)%Z by nomega.
+        transitivity (x0 * 0)%Z.
+
+        + apply Z.mul_le_mono_nonneg_l; try nomega.
+        + apply Z.mul_le_mono_nonpos_r; try nomega.
+
+      - apply trans4max_0.
+        replace 0%Z with (0*0)%Z by nomega.
+        transitivity (x0 * 0)%Z.
+
+        + apply Z.mul_le_mono_nonpos_l; try nomega.
+        + apply Z.mul_le_mono_nonneg_r; try nomega.
+
+      - apply trans4max_a.
+        apply Z.mul_le_mono_nonpos; try nomega.
+    Qed.
+  End BoundedMul.
+
+  Inductive BoundedZ :=
+    | boundedZ: forall (x low high: Z),
+      (low <= x)%Z -> (x <= high)%Z -> BoundedZ.
+
+  Definition bprojZ (x: BoundedZ) :=
+    match x with
+    | boundedZ x0 low0 high0 plow0 phigh0 => x0
+    end.
+
+  Definition bZAdd (a b: BoundedZ): BoundedZ.
+    refine match a with
+    | boundedZ x0 low0 high0 plow0 phigh0 =>
+      match b with
+      | boundedZ x1 low1 high1 plow1 phigh1 =>
+        boundedZ (x0 + x1) (low0 + low1) (high0 + high1) _ _
+      end
+    end; abstract nomega.
+  Defined.
+
+  Definition bZSub (a b: BoundedZ): BoundedZ.
+    refine match a with
+    | boundedZ x0 low0 high0 plow0 phigh0 =>
+      match b with
+      | boundedZ x1 low1 high1 plow1 phigh1 =>
+        boundedZ (x0 - x1) (low0 - high1) (high0 - low1) _ _
+      end
+    end; abstract nomega.
+  Defined.
+
+  Definition bZMul (a b: BoundedZ): BoundedZ.
+    refine match a with
+    | boundedZ x0 low0 high0 plow0 phigh0 =>
+      match b with
+      | boundedZ x1 low1 high1 plow1 phigh1 =>
+        boundedZ (x0 * x1)
+          (min4 (low0 * low1) (low0 * high1)
+                (high0 * low1) (high0 * high1))
+          (max4 (low0 * low1) (low0 * high1)
+                (high0 * low1) (high0 * high1))
+          _ _
+      end
+    end; try apply bZMul_min; try apply bZMul_max; try assumption.
+  Defined.
+
+  Definition bZShiftr (a: BoundedZ) (k: nat): BoundedZ.
+    assert (forall k, 2 ^ (Z.of_nat k) > 0)%Z as H by abstract (
+      intro m;
+      rewrite <- two_p_equiv;
+      apply two_p_gt_ZERO;
+      induction m; try reflexivity;
+      rewrite Nat2Z.inj_succ;
+      nomega).
+
+    refine match a with
+    | boundedZ x low high plow phigh =>
+      boundedZ (Z.shiftr x (Z.of_nat k))
+               (Z.shiftr low (Z.of_nat k))
+               (Z.succ (Z.shiftr high (Z.of_nat k))) _ _
+    end.
+
+    - abstract (
+        repeat rewrite Z.shiftr_div_pow2;
+        try apply Nat2Z.is_nonneg;
+        apply Z_div_le; try assumption;
+        try apply H).
+
+    - abstract (
+        apply Z.lt_succ_r;
+        repeat rewrite Z.shiftr_div_pow2;
+        try apply Nat2Z.is_nonneg;
+        apply Z.lt_lt_succ_r;
+        apply Z.lt_succ_r;
+        apply Z_div_le;
+        try apply H;
+        try assumption).
+  Qed.
+
+  Definition bZMask (a: BoundedZ) (k: nat): BoundedZ.
+    assert (0 < 2 ^ Z.of_nat k)%Z as Hk by (
+      induction k;
+      try abstract (vm_compute; reflexivity);
+      rewrite Nat2Z.inj_succ;
+      rewrite <- two_p_equiv;
+      apply Z.gt_lt;
+      apply two_p_gt_ZERO;
+      apply Z.le_le_succ_r;
+      apply Nat2Z.is_nonneg).
+
+    refine match a with
+    | boundedZ x low high plow phigh =>
+      boundedZ (Z.land x (Z.ones (Z.of_nat k)))
+               (Z.of_N 0%N)
+               (Z.of_N (Npow2 k)) _ _
+    end.
+
+    - repeat rewrite Z.land_ones;
+        try apply Nat2Z.is_nonneg.
+
+      abstract (
+        apply (Z.mod_pos_bound x) in Hk; destruct Hk;
+        induction k; simpl in *; assumption).
+
+    - repeat rewrite Z.land_ones;
+        try apply Nat2Z.is_nonneg.
+
+      abstract (
+        rewrite Npow2_N;
+        rewrite N2Z.inj_pow; simpl;
+        apply (Z.mod_pos_bound x) in Hk; destruct Hk;
+        apply Z.lt_le_incl;
+        induction k; simpl in *; assumption).
+  Qed.
+End BoundedZ.
+
+Section BoundedN.
+
+  Inductive BoundedN :=
+    | boundedN: forall (x low high: N),
+      (low <= x)%N -> (x < high)%N -> BoundedN.
+
+  Definition bprojN (x: BoundedN) :=
+    match x with
+    | boundedN x0 low0 high0 plow0 phigh0 => x0
+    end.
+
+  Definition bNAdd (a b: BoundedN): BoundedN.
+    refine match a with
+    | boundedN x0 low0 high0 plow0 phigh0 =>
+      match b with
+      | boundedN x1 low1 high1 plow1 phigh1 =>
+        boundedN (x0 + x1) (low0 + low1) (high0 + high1) _ _
+      end
+    end.
+
+    - abstract (apply N.add_le_mono; assumption).
+    - abstract nomega.
+  Defined.
+
+  Definition bNSub (a b: BoundedN): BoundedN.
+    refine match a with
+    | boundedN x0 low0 high0 plow0 phigh0 =>
+      match b with
+      | boundedN x1 low1 high1 plow1 phigh1 =>
+        boundedN (x0 - x1) (low0 - high1) (N.succ (high0 - low1)) _ _
+      end
+    end.
+
+    - transitivity (x0 - high1)%N.
+
+      + apply N.sub_le_mono_r; assumption.
+      + apply N.sub_le_mono_l; apply N.lt_le_incl; assumption.
+
+    - apply N.lt_succ_r; transitivity (high0 - x1)%N.
+
+      + apply N.sub_le_mono_r; apply N.lt_le_incl; assumption.
+      + apply N.sub_le_mono_l; assumption.
+
+  Defined.
+
+  Definition bNMul (a b: BoundedN): BoundedN.
+    refine match a with
+    | boundedN x0 low0 high0 plow0 phigh0 =>
+      match b with
+      | boundedN x1 low1 high1 plow1 phigh1 =>
+        boundedN (x0 * x1)%N (low0 * low1)%N (high0 * high1)%N _ _
+      end
+    end; abstract (
+      try apply N.mul_le_mono_nonneg;
+      try apply N.mul_lt_mono_nonneg;
+        try assumption;
+        try apply N_ge_0).
+  Qed.
+
+  Definition bNShiftr (a: BoundedN) (k: nat): BoundedN.
+    assert (forall k, 2 ^ (N.of_nat k) > 0)%N as H by abstract (
+      intros;
+      rewrite <- Npow2_N;
+      apply N.lt_gt;
+      apply Npow2_gt0).
+
+    refine match a with
+    | boundedN x low high plow phigh =>
+      boundedN (N.shiftr x (N.of_nat k))
+               (N.shiftr low (N.of_nat k))
+               (N.succ (N.shiftr high (N.of_nat k))) _ _
+    end.
+
+    - repeat rewrite N.shiftr_div_pow2.
+      apply N.div_le_mono; try assumption.
+      pose proof (H k) as H0.
+      induction ((2 ^ N.of_nat k)%N);
+        [inversion H0; intuition |].
+      apply N.neq_0_lt_0; apply N.gt_lt; assumption.
+
+    - apply N.lt_succ_r.
+      repeat rewrite N.shiftr_div_pow2.
+      apply N.div_le_mono; [|apply N.lt_le_incl; assumption].
+      pose proof (H k) as H0.
+      induction ((2 ^ N.of_nat k)%N);
+        [inversion H0; intuition |].
+      apply N.neq_0_lt_0; apply N.gt_lt; assumption.
+  Defined.
+
+  Definition bNMask (a: BoundedN) (k: nat): BoundedN.
+    assert (forall k, 0 < 2 ^ (N.of_nat k))%N as H by abstract (
+      intros;
+      rewrite <- Npow2_N;
+      apply Npow2_gt0).
+
+    refine match a with
+    | boundedN x low high plow phigh =>
+      boundedN (N.land x (N.ones (N.of_nat k)))
+               0%N
+               (Npow2 k) _ _
+    end.
+
+    - repeat rewrite N.land_ones;
+        apply N_ge_0.
+
+    - repeat rewrite N.land_ones.
+
+      abstract (
+        rewrite Npow2_N;
+        pose proof (N.mod_bound_pos x (2 ^ N.of_nat k)%N (N_ge_0 _) (H k))
+          as H0; destruct H0;
+        assumption).
+  Defined.
+
+End BoundedN.
+
+Section BoundedWord.
+  Context {n: nat}.
+
+  Section BoundedSub.
+    Lemma NToWord_Npow2: wzero n = NToWord n (Npow2 n).
+    Proof.
+      induction n as [|n0].
+
+      + repeat rewrite shatter_word_0; reflexivity.
+
+      + unfold wzero in *; simpl in *.
+        rewrite IHn0; simpl.
+        induction (Npow2 n0); simpl; reflexivity.
+    Qed.
+
+    Lemma bWSub_lem0: forall (x0 x1: word n) (low0 high1: N),
+      (low0 <= wordToN x0)%N -> (wordToN x1 < high1)%N -> 
+      (low0 - high1 <= & (x0 ^- x1))%N.
+    Proof.
+      intros.
+
+      destruct (Nge_dec (wordToN x1) 1)%N as [e|e].
+      destruct (Nge_dec (wordToN x1) (wordToN x0)).
+
+      - unfold wminus, wneg.
+        assert (low0 < high1)%N. {
+          apply (N.le_lt_trans _ (wordToN x0) _); [assumption|].
+          apply (N.le_lt_trans _ (wordToN x1) _); [apply N.ge_le|]; assumption.
+        }
+
+        replace (low0 - high1)%N with 0%N; [apply N_ge_0|].
+        symmetry.
+        apply N.sub_0_le.
+        apply N.lt_le_incl.
+        assumption.
+
+        - transitivity (wordToN x0 - wordToN x1)%N.
+
+          + transitivity (wordToN x0 - high1)%N.
+
+            * apply N.sub_le_mono_r; assumption.
+
+            * apply N.sub_le_mono_l; apply N.lt_le_incl; assumption.
+
+          + assert (& x0 - & x1 < Npow2 n)%N. {
+              transitivity (wordToN x0);
+                try apply word_size_bound;
+                apply N.sub_lt.
+
+              + apply N.lt_le_incl; assumption.
+
+              + nomega.
+            }
+
+            assert (& x0 - & x1 + & x1 < Npow2 n)%N. {
+              replace (wordToN x0 - wordToN x1 + wordToN x1)%N
+                with (wordToN x0) by nomega.
+              apply word_size_bound.
+            }
+
+            assert (x0 = NToWord n (wordToN x0 - wordToN x1) ^+ x1) as Hv. {
+              apply NToWord_equal.
+              rewrite <- wordize_plus; rewrite wordToN_NToWord;
+                try assumption.
+              nomega.
+            }
+
+            apply N.eq_le_incl.
+            rewrite Hv.
+            unfold wminus.
+            rewrite <- wplus_assoc.
+            rewrite wminus_inv.
+            rewrite (wplus_comm (NToWord n (wordToN x0 - wordToN x1)) (wzero n)).
+            rewrite wplus_unit.
+            rewrite <- wordize_plus; [nomega|].
+            rewrite wordToN_NToWord; assumption.
+
+      - unfold wminus, wneg.
+        assert (wordToN x1 = 0)%N as e' by nomega.
+        rewrite e'.
+        replace (Npow2 n - 0)%N with (Npow2 n) by nomega.
+        rewrite <- NToWord_Npow2.
+
+        erewrite <- wordize_plus;
+          try rewrite wordToN_zero;
+          replace (wordToN x0 + 0)%N with (wordToN x0)%N by nomega;
+          try apply word_size_bound.
+
+        transitivity low0; try assumption.
+        apply N.le_sub_le_add_r.
+        apply N.le_add_r.
+    Qed.
+
+    Lemma bWSub_lem1: forall (x0 x1: word n) (low1 high0: N),
+      (low1 <= wordToN x1)%N -> (wordToN x0 < high0)%N -> 
+      (& (x0 ^- x1) < N.succ (high0 + Npow2 n - low1))%N.
+    Proof.
+      intros; unfold wminus.
+      destruct (Nge_dec (wordToN x1) 1)%N as [e|e].
+      destruct (Nge_dec (wordToN x0) (wordToN x1)).
+
+      - apply N.lt_succ_r.
+        assert (& x0 - & x1 < Npow2 n)%N. {
+          transitivity (wordToN x0);
+          try apply word_size_bound;
+          apply N.sub_lt.
+
+          + apply N.ge_le; assumption.
+
+          + nomega.
+        }
+
+        assert (& x0 - & x1 + & x1 < Npow2 n)%N. {
+          replace (wordToN x0 - wordToN x1 + wordToN x1)%N
+            with (wordToN x0) by nomega.
+          apply word_size_bound.
+        }
+
+        assert (x0 = NToWord n (wordToN x0 - wordToN x1) ^+ x1) as Hv. {
+          apply NToWord_equal.
+          rewrite <- wordize_plus; rewrite wordToN_NToWord;
+          try assumption.
+          nomega.
+        }
+
+        rewrite Hv.
+        rewrite <- wplus_assoc.
+        rewrite wminus_inv.
+        rewrite wplus_comm.
+        rewrite wplus_unit.
+        rewrite wordToN_NToWord.
+
+        + transitivity (wordToN x0 - low1)%N.
+
+          * apply N.sub_le_mono_l; assumption.
+
+          * apply N.sub_le_mono_r.
+            transitivity high0; [apply N.lt_le_incl; assumption|].
+            replace' high0 with (high0 + 0)%N at 1 by nomega.
+            apply N.add_le_mono_l.
+            apply N_ge_0.
+
+        + transitivity (wordToN x0); try apply word_size_bound.
+            nomega.
+
+      - rewrite <- wordize_plus; [apply N.lt_succ_r|].
+
+        + transitivity (high0 + (wordToN (wneg x1)))%N.
+
+          * apply N.add_le_mono_r; apply N.lt_le_incl; assumption.
+
+          * unfold wneg.
+            rewrite wordToN_NToWord; [|abstract (
+              apply N.sub_lt;
+              try apply N.lt_le_incl;
+              try apply word_size_bound;
+              nomega )].
+
+            rewrite N.add_sub_assoc; [|abstract (
+              try apply N.lt_le_incl;
+              try apply word_size_bound)].
+
+            apply N.sub_le_mono_l.
+            assumption.
+
+        + unfold wneg.
+
+          rewrite wordToN_NToWord; [|abstract (
+            apply N.sub_lt;
+            try apply N.lt_le_incl;
+            try apply word_size_bound;
+            nomega )].
+
+          replace (wordToN x0 + (Npow2 n - wordToN x1))%N
+            with (Npow2 n - (wordToN x1 - wordToN x0))%N.
+
+          * apply N.sub_lt; try nomega.
+            transitivity (wordToN x1); [apply N.le_sub_l|].
+            apply N.lt_le_incl.
+            apply word_size_bound.
+
+          * apply N.add_sub_eq_l.
+            rewrite <- N.add_sub_swap;
+                [|apply N.lt_le_incl; assumption].
+            rewrite (N.add_comm (wordToN x0)).
+            rewrite N.add_assoc.
+            rewrite N.add_sub_assoc;
+                [|apply N.lt_le_incl; apply word_size_bound].
+            rewrite N.add_sub.
+            rewrite N.add_comm.
+            rewrite N.add_sub.
+            reflexivity.
+
+      - apply N.lt_succ_r.
+        assert (wordToN x1 = 0)%N as e' by nomega.
+        assert (NToWord n (wordToN x1) = NToWord n 0%N) as E by
+            (rewrite e'; reflexivity).
+        rewrite NToWord_wordToN in E.
+        simpl in E; rewrite wzero'_def in E.
+        rewrite E.
+        unfold wneg.
+        rewrite wordToN_zero.
+        rewrite N.sub_0_r.
+        rewrite <- NToWord_Npow2.
+        rewrite wplus_comm.
+        rewrite wplus_unit.
+        transitivity high0.
+
+        + apply N.lt_le_incl.
+          assumption.
+
+        + rewrite <- N.add_sub_assoc.
+
+          * replace high0 with (high0 + 0)%N by nomega.
+            apply N.add_le_mono; [|apply N_ge_0].
+            apply N.eq_le_incl.
+            rewrite N.add_0_r.
+            reflexivity.
+
+          * transitivity (wordToN x1);
+            [ assumption
+            | apply N.lt_le_incl;
+                apply word_size_bound].
+
+    Qed.
+  End BoundedSub.
+
+  Inductive BoundedWord :=
+    | boundedWord: forall (x: word n) (low high: N) (overflowed: bool),
+      (low <= wordToN x)%N -> (wordToN x < high)%N -> BoundedWord.
+
+  Definition bprojW (x: BoundedWord) :=
+    match x with
+    | boundedWord x0 _ _ _ _ _ => x0
+    end.
+
+  Definition bWAdd (a b: BoundedWord): BoundedWord.
+    refine match a with
+    | boundedWord x0 low0 high0 o0 plow0 phigh0 =>
+      match b with
+      | boundedWord x1 low1 high1 o1 plow1 phigh1 =>
+        if (overflows n (high0 + high1))
+        then boundedWord (x0 ^+ x1) 0%N (high0 + high1) (orb o0 o1) _ _
+        else boundedWord (x0 ^+ x1) (low0 + low1) (high0 + high1) true _ _
+      end
+    end; try abstract (
+      apply (N.le_lt_trans _ (wordToN x0 + wordToN x1)%N _);
+        try apply plus_le;
+        abstract nomega).
+
+    - apply N_ge_0.
+
+    - erewrite <- wordize_plus';
+        try eassumption;
+        try abstract nomega.
+
+      + apply N.add_le_mono; assumption.
+
+      + abstract (apply N.lt_le_incl; nomega).
+  Qed.
+
+  Definition bWSub (a b: BoundedWord): BoundedWord.
+    refine match a with
+    | boundedWord x0 low0 high0 o0 plow0 phigh0 =>
+      match b with
+      | boundedWord x1 low1 high1 o1 plow1 phigh1 =>
+        let upper_bound :=
+          if (Nge_dec high0 (Npow2 n))
+          then Npow2 n
+          else if (Nge_dec high1 (Npow2 n))
+               then Npow2 n
+               else (N.succ (high0 + Npow2 n - low1)) in
+
+        if (Nge_dec low0 high1)
+        then boundedWord (x0 ^- x1) (low0 - high1)%N upper_bound (orb o0 o1) _ _
+        else boundedWord (x0 ^- x1) 0%N upper_bound (orb o0 o1) _ _
+      end
+    end; abstract (unfold upper_bound; try apply N_ge_0;
+      destruct (Nge_dec high0 (Npow2 n)), (Nge_dec high1 (Npow2 n));
+      repeat match goal with
+      | [|- (_ - ?x <= wordToN _)%N] => apply bWSub_lem0
+      | [|- (wordToN _ < N.succ (?x + _ - _))%N] => apply bWSub_lem1
+      | [|- (wordToN _ < Npow2 _)%N] => apply word_size_bound
+      | [|- (0 <= _)%N] => apply N_ge_0
+      end; assumption).
+  Qed.
+
+  Definition bWMul (a b: BoundedWord): BoundedWord.
+    refine match a with
+    | boundedWord x0 low0 high0 o0 plow0 phigh0 =>
+      match b with
+      | boundedWord x1 low1 high1 o1 plow1 phigh1 =>
+        if (overflows n (high0 * high1))
+        then boundedWord (x0 ^* x1)%N 0%N (high0 * high1)%N true _ _
+        else boundedWord (x0 ^* x1)%N (low0 * low1)%N (high0 * high1)%N (orb o0 o1) _ _
+      end
+    end.
+
+    - apply N_ge_0.
+
+    - apply (N.le_lt_trans _ (wordToN x0 * wordToN x1)%N _); [apply mult_le|].
+      apply N.mul_lt_mono; assumption.
+
+    - rewrite <- wordize_mult.
+
+      + apply N.mul_le_mono; assumption.
+
+      + transitivity (high0 * high1)%N; [|assumption].
+        apply N.mul_lt_mono; assumption.
+
+    - apply (N.le_lt_trans _ (wordToN x0 * wordToN x1)%N _); [apply mult_le|].
+      apply N.mul_lt_mono; assumption.
+  Qed.
+
+  Definition bWShiftr (a: BoundedWord) (k: nat): BoundedWord.
+    assert (forall k, 2 ^ (N.of_nat k) > 0)%N as H by abstract (
+      intros;
+      rewrite <- Npow2_N;
+      apply N.lt_gt;
+      apply Npow2_gt0).
+
+    refine match a with
+    | boundedWord x low high o plow phigh =>
+      boundedWord (extend _ (shiftr x k))
+        (N.shiftr low (N.of_nat k))
+        (N.succ (N.shiftr high (N.of_nat k))) o _ _
+    end.
+
+    - unfold extend; rewrite wordToN_convS.
+
+      rewrite wordToN_zext.
+      rewrite <- wordize_shiftr.
+      rewrite <- Nshiftr_equiv_nat.
+      repeat rewrite N.shiftr_div_pow2.
+      apply N.div_le_mono; try assumption.
+      pose proof (H k) as H0.
+      induction ((2 ^ N.of_nat k)%N);
+        [inversion H0; intuition |].
+      apply N.neq_0_lt_0; apply N.gt_lt; assumption.
+
+    - unfold extend; rewrite wordToN_convS.
+      rewrite wordToN_zext.
+      rewrite Nshiftr_equiv_nat.
+      eapply N.lt_le_trans; [apply shiftr_bound; eassumption|].
+      try apply N.eq_le_incl.
+      try eassumption; reflexivity.
+
+    (* TODO(rsloan): how do we fix this? *)
+    Unshelve.
+    reflexivity.
+  Qed.
+
+  Definition bWMask (a: BoundedWord) (k: nat): BoundedWord.
+    refine match a with
+    | boundedWord x low high o plow phigh =>
+      boundedWord (mask k x) 0%N (Npow2 k) o _ _
+    end; [apply N_ge_0 | apply mask_bound].
+  Qed.
+End BoundedWord.
